src/trees.v
@@ -1,0 +1,165 @@
+From mathcomp Require Import ssreflect ssrbool ssrfun.
+From mathcomp Require Import eqtype ssrnat seq bigop choice.
+From ipcssr Require Import prelude.
+
+Inductive tree A := TNode of A & seq (tree A).
+Arguments TNode [A].
+
+Section Tree.
+Context {A : Type}.
+
+(* a leaf is a node with an empty list *)
+Definition lf a : tree A := TNode a [::].
+
+Lemma tree_ind' (P : tree A -> Prop) :
+  (forall a l, all_prop P l -> P (TNode a l)) ->
+  forall t, P t.
+Proof.
+move=> indu; fix H 1.
+elim => a l; apply indu.
+by elim: l.
+Qed.
+
+Lemma tree_rec' (P : tree A -> Type) :
+  (forall a l, all_type P l -> P (TNode a l)) ->
+  forall t, P t.
+Proof.
+move=>indu; fix H 1.
+elim => a l; apply: indu.
+by elim: l.
+Qed.
+
+Fixpoint height (t : tree A) : nat :=
+  let: TNode _ l := t in (\max_(i <- map height l) i).+1.
+
+Definition root (T : tree A) : A := let: TNode w _ := T in w.
+
+Definition children_of_node (t : tree A) :=
+  let: TNode _ l := t in l.
+
+End Tree.
+
+Section EncodeDecodeTree.
+Variable A : Type.
+
+Fixpoint encode_tree (t : tree A) : GenTree.tree A :=
+  match t with
+  | TNode a [::] => GenTree.Leaf a
+  | TNode a l => GenTree.Node O(*dummy*) (GenTree.Leaf a :: map encode_tree l)
+  end.
+
+Fixpoint decode_tree (t : GenTree.tree A) : option (tree A) :=
+  match t with
+  | GenTree.Leaf a => Some (TNode a [::])
+  | GenTree.Node _ (GenTree.Leaf h :: l) => Some (TNode h (pmap decode_tree l))
+  | GenTree.Node _ _ => None
+  end.
+
+Lemma pcancel_tree : pcancel encode_tree decode_tree.
+Proof.
+elim/(@tree_ind' A) => a [//|b s /= [-> H2 /=]]; congr (Some (TNode _ (_ :: _))).
+elim: s H2 => // c s IH /= [-> K2 /=]; by rewrite IH.
+Qed.
+
+End EncodeDecodeTree.
+
+Definition tree_eqMixin (A : eqType) := PcanEqMixin (@pcancel_tree A).
+Canonical tree_eqType (A : eqType) := Eval hnf in EqType _ (@tree_eqMixin A).
+
+(* we formulate the rest of the theory with decidable equality for convenience *)
+(* this is because we only use it for Kripke trees whose elements are *)
+(* sets (AVL-maps) of atoms, which implies dec. eq. *)
+Section TreeEq.
+Context {A : eqType}.
+
+Fixpoint successor (t1 t2 : tree A) : bool :=
+  (t1 == t2) || has (successor t1) (children_of_node t2).
+
+Lemma successor_refl : reflexive successor.
+Proof. by case=>/= a ts; rewrite eqxx. Qed.
+
+Lemma successor_trans : transitive successor.
+Proof.
+move=>t2 t1; elim/(@tree_ind' A)=>a3 ts3 /= IH H1.
+case/orP=>[/eqP E2|]; first by rewrite E2 in H1.
+case/hasP=>z Hz Pz; apply/orP; right; apply/hasP; exists z=>//.
+by move: H1 Pz; apply: (all_prop_mem IH).
+Qed.
+
+Lemma child_ind (P : tree A -> Prop) :
+  (forall a, P (lf a)) ->
+  (forall t0 t1, successor t0 t1 -> P t0 -> P t1) ->
+  forall t, P t.
+Proof.
+move=>Pl Pc t.
+apply: tree_ind'=>a [_ |h ts /= [Ph Pts]]; first by apply: Pl.
+by apply: (Pc h)=>//=; rewrite successor_refl orbT.
+Qed.
+
+Fixpoint mem_tree (t : tree A) : pred A :=
+  let: TNode x l := t in
+  fun a => (a == x) || has (mem_tree^~ a) l.
+
+Definition tree_eqclass := tree A.
+Identity Coercion tree_of_eqclass : tree_eqclass >-> tree.
+Coercion pred_of_tree (t : tree_eqclass) : {pred A} := mem_tree t.
+
+Canonical tree_predType := PredType (pred_of_tree : tree A -> pred A).
+(* The line below makes mem_tree a canonical instance of topred. *)
+Canonical mem_tree_predType := PredType mem_tree.
+
+Lemma in_tnode a t ts : (t \in TNode a ts) = (t == a) || has (fun q => t \in q) ts.
+Proof. by []. Qed.
+
+Lemma successor_subset (t t0 : tree A) :
+  successor t t0 -> {subset t <= t0}.
+Proof.
+elim/(@tree_ind' A): t0=>a0 ts0 /= IH.
+case/orP=>[/eqP->|] //; case/hasP=>/= z Hz Sz.
+have H: {subset t <= z} by apply: (all_prop_mem IH).
+move=>q /H Hq; rewrite in_tnode /=.
+by apply/orP; right; apply/hasP; exists z.
+Qed.
+
+Context {I : Set} {P : A -> I -> bool}.
+
+Fixpoint Is_Monotone_Tree (t : tree A) : Prop :=
+  let: TNode x l := t in
+  all_prop (fun t => (forall i, P x i ==> P (root t) i)
+                  /\ Is_Monotone_Tree t) l.
+
+Lemma successor_is_monotone_tree (t t0 : tree A) :
+  successor t0 t -> Is_Monotone_Tree t -> Is_Monotone_Tree t0.
+Proof.
+elim/(@tree_ind' A): t=>a ts /= IH.
+case/orP=>[/eqP->|] //; case/hasP=>/= z Hz Sz H.
+apply: (all_prop_mem (x:=z) IH)=>{t0 Sz IH}//.
+by case: (all_prop_mem H Hz).
+Qed.
+
+Definition Is_Monotone (t : tree A) : Prop :=
+  forall t0 t1 : tree A,
+  successor t1 t0 -> successor t0 t ->
+  forall i : I, P (root t0) i ==> P (root t1) i.
+
+Lemma successor_is_monotone (t t0 : tree A) :
+  successor t0 t -> Is_Monotone t -> Is_Monotone t0.
+Proof.
+move=>S0; rewrite /Is_Monotone => H t1 t2 S21 S10.
+by apply: H=>//; apply/successor_trans/S0.
+Qed.
+
+Lemma is_monotone_tree_is_monotone t :
+  Is_Monotone_Tree t -> Is_Monotone t.
+Proof.
+rewrite /Is_Monotone=>H t0 t1 S10 S0 i.
+move: (successor_is_monotone_tree _ _ S0 H)=>{S0 H}.
+elim/(@tree_ind' A): t0 S10=>a0 ts0 /= IH.
+case/orP=>[/eqP-> _|] /=; first by apply: implybb.
+case/hasP=>/= z Hz Sz H.
+case: (all_prop_mem H Hz)=>Hi Hmz.
+apply: (implyb_trans (y:=P (root z) i))=>//.
+by apply: (all_prop_mem IH).
+Qed.
+
+End TreeEq.
